<section xml:id="sec-cyclic-subspaces">
	<title>Cyclic subspaces</title>
	<definition xml:id="def-principal-vector">
		<title>(Principal vector and its order)</title>
		<statement>
			<p>
				Let <m>V</m> be a finite-dimensional vector space over a field <m>F</m>. A nonzero vector <m>e\in V</m> is said to be a <term>principal vector of an <m>F</m>-linear map <m>T\colon V\to V</m> with an eigenvalue <m>\lambda\in F</m></term> if there exists a natural number <m>n</m> such that <m>(T-\lambda\unit_V)^n(e)=0</m>.
			</p>
			<p>
				The least natural number <m>m</m> such that <m>(T-\lambda\unit_V)^m(e)=0</m> is called the <term>order</term> of <m>e</m>.
			</p>
			<p>
				A principal vector of <m>T</m> with an eigenvalue <m>\lambda</m> is also called a <term>generalized eigenvector with eigenvalue <m>\lambda</m></term>.
			</p>
		</statement>
	</definition>
	<remark>
		<statement>
			An eigenvector is a principal vector of order <m>1</m>.
		</statement>
	</remark>
	<example xml:id="illustrative-example-principla-vector"><title>(An illustrative example)</title>
		Let <m>T\colon\R^2\to\R^2</m> be a linear map corresponding to a matrix <m>A=\begin{pmatrix}1\amp 1\\0\amp 1\end{pmatrix}</m> (see <xref ref="iso-matrices-Hom"/>). We have <me>(T-\unit_V)(e_1)=0\quad\text{and}\quad(T-\unit_V)(e_2)=e_1.</me>
		Thus, <me>(T-\unit_V)^2(e_2)=0.</me>
		Therefore, <m>e_1</m> is a principal vector of <m>T</m> with eigenvalue <m>1</m> and its order is <m>1</m>. While <m>e_2\in\R^2</m> is a principal vector of <m>T</m> with an eigenvalue <m>1</m>, and its order is <m>2</m>. Since vectors <m>w_1=e_2,w_2=(T-\unit_V)(e_2)</m> are <m>\R</m>-linearly independent, they form a basis of <m>\R^2</m>. Furthermore, since <m>T(w_1)=w_1+w_2</m> and <m>(T-\unit_V)(w_2)=(T-\unit_V)^2(e_2)=0</m>, the matrix of <m>T</m> with respect to an ordered basis <m>(w_1,w_2)</m> is 
		<me>\begin{pmatrix}1\amp0\\1\amp1\end{pmatrix}.</me>
	</example>
	<definition xml:id="def-cyclic-subspace">
		<title>(Cyclic subspace)</title>
		<statement>
			Let <m>V</m> be a finite-dimensional vector space over a field <m>F</m>. Consider a nonzero (principal) vector <m>e\in V</m>, a scalar <m>\lambda\in F</m> such that <m>(T-\lambda\unit_V)^n(e)=0</m>. Suppose that <m>m</m> is the least natural number such that <m>(T-\lambda\unit_V)^m(e)=0</m>. The subspace of <m>V</m> generated by 
			<me>e,(T-\lambda\unit_V)(e),(T-\lambda\unit_V)^2(e),\ldots,(T-\lambda\unit_V)^{m-1}(e)</me> is called the <term>cyclic subspace generated by <m>e</m></term>.
		</statement>
	</definition>
	<proposition xml:id="dim-cyclic-subspace">
		<statement>
			Let <m>V</m> be a finite-dimensional vector space over a field <m>F</m> and let <m>T\colon V\to V</m> be an <m>F</m>-linear map. The cyclic subspace <m>W</m> generated by the principal vector <m>e</m> of order <m>m</m> with an eigenvalue <m>\lambda</m> is invariant under <m>T</m> and <m>\dim_FW=m</m>.
		</statement>
	</proposition>
	<proof>
		<p>
			We first compute the dimension of <m>W</m>. By <xref ref="def-cyclic-subspace"/>, the subspace <m>W</m> is spanned by <me>e,\;(T-\lambda\unit_V)(e),\;(T-\lambda\unit_V)^2(e),\ldots,(T-\lambda\unit_V)^{m-1}(e).</me> Hence, <m>\dim_FW\leq m</m>. We show that <m>\left\{(T-\lambda\unit_V)^i(e)\right\}_{i=0}^{m-1}</m> is linearly independent. Suppose that 
			<me>a_0e+a_1(T-\lambda\unit_V)(e)+\cdots+a_{m-1}(T-\lambda\unit_V)^{m-1}(e)=0.</me> Since <m>(T-\lambda\unit_V)^m(e)=0</m>, we get that <m>(T-\lambda\unit_V)^r(e)=0</m> for any <m>r\geq m</m>. Hence, the linear map <m>(T-\lambda\unit_V)^{m-1}</m> evaluated at the above expression gives
			<me>a_0(T-\lambda\unit_V)^{m-1}(e)=0.</me> As <m>(T-\lambda\unit_V)^{m-1}(e)\neq 0</m>, we have <m>a_0=0</m>. Therefore we are left with
			<me>a_1(T-\lambda\unit_V)(e)+\cdots+a_{m-1}(T-\lambda\unit_V)^{m-1}(e)=0.</me> Now we apply <m>(T-\lambda\unit_V)^{m-2}</m> to the above expression, and argueing as above, we obtain <m>a_1=0</m>. Continuing in this way we get that <m>a_i=0</m> for all <m>i</m>. This shows that <m>\left\{(T-\lambda\unit_V)^i\right\}_{i=0}^{m-1}</m> is a maximal linearly independent subset of <m>W</m>, i.e., it is a basis of <m>W</m>. Thus <m>\dim_FW=m</m>.
		</p>
		<p>
			We now show that <m>W</m> is invariant under <m>T</m>. We rename the basis vectors of <m>W</m> obtained above as follows.
			<me>w_1=e,\;w_2=(T-\lambda\unit_V)(e),\;w_3=(T-\lambda\unit_V)^2(e),\;\ldots,\;w_m=(T-\lambda\unit_V)^{m-1}(e)</me>
			Therefore we have 
			<me>(T-\lambda\unit_V)(w_i)=w_{i+1}\quad\text{for}\;1\leq i\leq m-1\quad\text{and}\quad (T-\lambda\unit_V)(w_m)=0.</me>
			In other words we have
			<me>T(w_i)=\lambda w_i+w_{i+1}\in W\quad\text{for}\;1\leq i\leq m-1\quad\text{and}\quad T(w_m)=\lambda w_m\in W.</me>
			This shows that <m>W</m> is invariant under <m>T</m>.
		</p>
	</proof>
	<remark xml:id="matrix-of-cyclic-subspace">
		<title>(Matrix of a cyclic subspace)</title>
		<statement>
			We keep the notation of the above <xref ref="dim-cyclic-subspace"/> and its proof. A matrix of <m>T|_W</m> with respect to the ordered basis <m>(w_1,w_2,\ldots,w_m)</m> is the matrix with all diagonal entries <m>\lambda</m>, all lower diagonal entries <m>1</m>, and all other entries <m>0</m>.
		</statement>
	</remark>
	<definition xml:id="def-Jordan-block">
		<title>(Jordan block)</title>
		The matrix of a cyclic subspace described in <xref ref="matrix-of-cyclic-subspace"/> is called the <term>Jordan block</term>.
		Thus Jordan block obtained in <xref ref="dim-cyclic-subspace
		"/> is the following lower triangular matrix.
		<me>
			J_\lambda=\begin{pmatrix}\lambda\amp 0\amp 0\amp\cdots\amp\cdots\amp 0\\1\amp\lambda\amp 0\amp\amp\amp 0\\0\amp 1\amp\lambda\amp\amp\amp\vdots\\\vdots\amp\amp\ddots\amp\ddots\amp\amp\vdots\\\vdots\amp\amp\amp\ddots\amp\lambda\amp 0\\0\amp 0\amp\cdots\amp\cdots\amp 1\amp \lambda\end{pmatrix}
		</me>
	</definition>
	<remark>
		<statement>
			The Jordan block of size <m>1,2,3</m> and <m>4</m> are, respectively
			<me>(\lambda),\;\begin{pmatrix}\lambda\amp\\1\amp\lambda\end{pmatrix},\;\begin{pmatrix}\lambda\amp \amp \\1\amp\lambda\amp \\\amp 1\amp\lambda\end{pmatrix},\;\begin{pmatrix}\lambda\amp\amp\amp\\1\amp\lambda\amp\amp\\\amp 1\amp\lambda\amp\\\amp\amp1\amp\lambda\end{pmatrix}.</me>
		</statement>
	</remark>
	<lemma>
		<statement>Let <m>J_\lambda\in M_n(F)</m> be a Jordan block.
		<ol>
			<li>The characteristic polynomial of <m>J_\lambda</m>, <m>\chi(t)=(t-\lambda)^n</m>.</li>
			<li>The trace of <m>J_\lambda</m>, <m>tr(J_\lambda)=n\lambda</m> and the determinant of <m>J_\lambda</m>, <m>\det(J_\lambda)=\lambda^n</m>.</li>
			<li>We have <m>\chi(t)=t^n-tr(J_\lambda)+\cdots+(-1)^n\det(J_\lambda)</m>.</li>
			<li>The minimal polynomial of <m>J_{\lambda}</m> coincides with the characteristic polynomial of <m>J_{\lambda}</m>.</li>
		</ol>
	</statement>
	</lemma>
	<proof>
		This follows from the properties of determinant. The third statement is consequence of <xref ref="symmetric-functions"/>. We now show the last statement. Suppose that <m>J_\lambda\in M_r(F)</m>. Note that <m>J_\lambda=\lambda I_r+J_0</m>. We have <m>J_0^k=0</m> for all <m>k\geq r</m>. Since <m>\lambda I_r\cdot J_0=J_0\cdot\lambda I_r</m> we have <me>\left(J_r-\lambda I_r\right)^k=J_0^k.</me> By <xref ref="minimal-poly-divides-annihilating-poly"/>, the minimal polynomial divides the characteristic polynomial hence, we get the result.
	</proof>
</section>